VisualProof/Rule/WirePrimitive/ContentFixtures.lean
@@ -3,7 +3,9 @@ import VisualProof.Rule.WirePrimitive.Content
 namespace VisualProof
 
 #check ConcreteWirePrimitive.AppliedSite.replacement_denotation
+#check ConcreteWirePrimitive.AppliedSite.universal_scope_transport
 #check WirePrimitive.AppliedSiteErasure.Result.inductionOn
+#check WirePrimitive.AppliedSiteErasure.Result.universal_scope_transport
 
 namespace WirePrimitive
 
